Progress of non-blocking bst verification

concurrency/bst_conc_nblocking_spec.v
@@ -6,6 +6,7 @@ Require Import bst.bst_conc_lemmas.
 Require Import VST.atomics.general_locks.
 Require Import VST.atomics.SC_atomics.
 Require Import Coq.Sets.Ensembles.
+Require Import VST.msl.iter_sepcon.
 
  Instance CompSpecs : compspecs. make_compspecs prog. Defined.
 Definition Vprog : varspecs. mk_varspecs prog. Defined.
@@ -32,97 +33,47 @@ Definition surely_malloc_spec :=
        LOCAL (temp ret_temp p)
        SEP (mem_mgr gv; malloc_token Ews t p * data_at_ Ews t p).
 
-(* Definition treebox_new_spec :=
-  DECLARE _treebox_new
-  WITH gv: globals
-  PRE  [  ]
-    PROP () LOCAL (gvars gv) SEP (mem_mgr gv)
-  POST [ tptr (tptr t_struct_tree_t) ]
-    EX v:val, EX lock:val, EX g:gname, EX g_root:gname,
-    PROP ()
-    LOCAL (temp ret_temp v)
-    SEP (mem_mgr gv; nodebox_rep g g_root lsh1 lock v;
-         (* leftover slice of pointer *) data_at_ lsh2 (tptr t_struct_tree_t) v;
-         malloc_token Ews (tptr t_struct_tree_t) v;
-         tree_rep2 g g_root E).
-
-*)
-(* Definition node_rep_inv_r' (R : (val * (own.gname * node_info) → mpred)) p gp  :=
-  sync_inv gp gsh1 (uncurry (uncurry R p)) .
-
-Definition node_rep_r (g:gname)  R arg : mpred := let '(np, (g_current,(r,g_info))) := arg in
-EX tp:val, atomic_int_at Ews tp np * in_tree g g_current *
-if eq_dec tp nullval then !!( g_info = Some None) && emp  else
-EX ga:gname, EX gb: gname, EX x: Z, EX vp: val, EX pa : val, EX pb : val,
-     !! (g_info = Some (Some(x,vp,ga,gb)) /\ Int.min_signed <= x <= Int.max_signed/\ is_pointer_or_null pa /\ is_pointer_or_null pb  /\ tc_val (atomic_int) vp 
-     /\ check_key_exist' x r) && data_at Ews t_struct_tree (Vint (Int.repr x),(vp,(pa,pb))) tp * malloc_token Ews t_struct_tree tp  *
-    |> node_rep_inv_r' R  pa ga * |> node_rep_inv_r' R  pb gb.
-
-Definition node_rep_closed g  := HORec (node_rep_r g ).
-
-Definition node_rep np g g_current r := node_rep_closed g (np, (g_current, r)) . 
-*)
-
-Fixpoint ghost_tree_rep (t: @ ghost_tree val ) (sh:share) (nb:val) (g_current:gname) (g:gname) range : mpred := 
+Fixpoint ghost_tree_rep (t: @ ghost_tree val ) (nb:val) (g_current:gname) (g:gname) range : mpred := 
  match t, range with
- | E_ghost , _ => atomic_ptr_at sh nullval nb * ghost_master1 (ORD := range_order)  (range,  (@None ghost_info)) g_current * in_tree g g_current
- | (T_ghost a ga x v b gb ), (l, r) => EX tp:val, EX lp, EX rp,  atomic_ptr_at sh tp nb * data_at Ews t_struct_tree (Vint (Int.repr x),(v,(lp,rp))) tp * ghost_master1 (ORD := range_order)  (range,  (@Some ghost_info (x,v,ga,gb))) g_current * in_tree g g_current *  ghost_tree_rep a sh lp ga g (l, Finite_Integer x) * ghost_tree_rep b sh rp gb g (Finite_Integer x, r)
+ | E_ghost , _ => atomic_ptr_at Ews nullval nb * ghost_master1 (ORD := range_order)  (range,  (@None ghost_info)) g_current 
+ | (T_ghost a ga lp x v b gb rp ), (l, r) =>  EX tp, EX sh, !!(readable_share sh) && atomic_ptr_at Ews tp nb * data_at sh t_struct_tree (Vint (Int.repr x),(v,(lp,rp))) tp * ghost_master1 (ORD := range_order)  (range,  (@Some ghost_info (x,v,ga,gb))) g_current * in_tree ga (l, Finite_Integer x) lp g * in_tree gb ( Finite_Integer x, r) rp g *  ghost_tree_rep a  lp ga g (l, Finite_Integer x) * ghost_tree_rep b rp gb g (Finite_Integer x, r)
  end.
- 
- 
-Fixpoint find_pure_tree (t : @ghost_tree val) : @tree val :=
-  match t with 
-  | E_ghost => E
-  | (T_ghost a ga x v  b gb) => T (find_pure_tree a) x v (find_pure_tree b)
-end.
 
-Fixpoint find_ghost_set (t : @ghost_tree val) (g:gname) : Ensemble gname :=
-  match t with 
-  | E_ghost => (Ensembles.Singleton _ g)
-  | (T_ghost a ga x v  b gb) => (Add _  (Union _ (find_ghost_set a ga) (find_ghost_set b gb)) g)
-end.
+Definition tree_rep2 (g:gname) (g_root: gname) (nb:val) (sh:share) (t: @tree val  ) : mpred := EX (tg:ghost_tree), !! (find_pure_tree tg = t) && ghost_tree_rep tg  nb g_root g (Neg_Infinity, Pos_Infinity) 
+                                                                                                                                 * bst_conc_lemmas.ghost_ref g (find_ghost_set tg g_root ( Neg_Infinity, Pos_Infinity) nb).
 
-Lemma find_ghost_set_finite : forall t g, finite (find_ghost_set t g).
-Proof.
-  induction t; intros; simpl.
-  - apply finite_singleton.
-  - apply finite_add, finite_union; auto.
-Qed.
-
-Definition tree_rep2 (g:gname) (g_root: gname) (nb:val) (sh:share) (t: @tree val  ) : mpred := EX (tg:ghost_tree), !! (find_pure_tree tg = t) && ghost_tree_rep tg sh nb g_root g (Neg_Infinity, Pos_Infinity) * bst_conc_lemmas.ghost_ref g (find_ghost_set tg g_root).
-
-Definition nodebox_rep (sh : share) (nb: val) :=  EX tp:val,  atomic_ptr_at sh tp nb.
+Definition nodebox_rep (sh : share) (nb: val) (g_root: gname) (g:gname)  :=  EX tp:val, EX lp: list val,  atomic_ptr_at sh tp nb * iter_sepcon ( fun p => EX sh1:share, data_at_ sh1 t_struct_tree p ) lp * in_tree g_root (Neg_Infinity, Pos_Infinity) nb g.
  
 
 Program Definition insert_spec :=
   DECLARE _insert
   ATOMIC TYPE (rmaps.ConstType ( val * share * Z * val * globals*gname* gname)) OBJ BST INVS base.empty base.top
-  WITH  b:_, sh:_, x: _, v:_, gv : _ , g:_, g_root:_
+  WITH  b, sh, x, v, gv, g, g_root
   PRE [  _tb OF (tptr atomic_ptr), _x OF tint,  _value OF (tptr tvoid) ]
           PROP (readable_share sh;Int.min_signed <= x <= Int.max_signed;  is_pointer_or_null v )
           LOCAL (temp _tb b; temp _x (Vint (Int.repr x)); temp _value v; gvars gv )
-          SEP  (mem_mgr gv; nodebox_rep sh b ) | (!!(sorted_tree BST)&&tree_rep2 g g_root b sh  BST )
+          SEP  (mem_mgr gv; nodebox_rep sh b g_root g ) | (!!(sorted_tree BST)&&tree_rep2 g g_root b sh  BST )
   POST[ tvoid  ]
         PROP ()
         LOCAL ()
-       SEP (mem_mgr gv) | (!!(sorted_tree (bst_conc_lemmas.insert x v BST))&&tree_rep2 g g_root  b sh (bst_conc_lemmas.insert x v BST) ). 
+       SEP (mem_mgr gv; nodebox_rep sh b g_root g) | (!!(sorted_tree (bst_conc_lemmas.insert x v BST))&&tree_rep2 g g_root  b sh (bst_conc_lemmas.insert x v BST) ). 
 
 Program Definition lookup_spec :=
   DECLARE _lookup
   ATOMIC TYPE (rmaps.ConstType ( val * share* Z * globals * gname * gname))
          OBJ BST INVS base.empty base.top
-  WITH b:_, sh:_, x:_, gv:_, g:_, g_root:_
+  WITH b, sh, x, gv, g, g_root
   PRE [_tb OF (tptr atomic_ptr), _x OF tint]
     PROP (
           Int.min_signed <= x <= Int.max_signed)
     LOCAL (temp _tb b; temp _x (Vint (Int.repr x)); gvars gv)
-    SEP  (mem_mgr gv; nodebox_rep sh b) |
+    SEP  (mem_mgr gv; nodebox_rep sh b g_root g) |
   (!! sorted_tree BST && tree_rep2 g g_root b sh BST)
   POST [tptr Tvoid]
     EX ret: val,
     PROP ()
     LOCAL (temp ret_temp ret)
-    SEP (mem_mgr gv; nodebox_rep sh b) |
+    SEP (mem_mgr gv; nodebox_rep sh b g_root g) |
         (!! (sorted_tree BST /\ ret = (bst_conc_lemmas.lookup nullval x BST)) && tree_rep2 g g_root b sh BST).
 
 Definition main_spec :=
@@ -139,6 +90,7 @@ Definition spawn_spec := DECLARE _spawn spawn_spec.
 Definition atomic_load_ptr_spec := DECLARE _atomic_load_ptr (atomic_load_ptr_spec atomic_ptr atomic_ptr_at).
 Definition atomic_store_ptr_spec := DECLARE _atomic_store_ptr (atomic_store_ptr_spec atomic_ptr atomic_ptr_at).
 Definition atomic_CAS_ptr_spec := DECLARE _atomic_CAS_ptr (atomic_CAS_ptr_spec atomic_ptr atomic_ptr_at).
+Definition make_atomic_ptr_spec := DECLARE _make_atomic_ptr ( make_atomic_ptr_spec atomic_ptr atomic_ptr_at).
 
 Definition Gprog : funspecs :=
     ltac:(with_library prog [acquire_spec; release2_spec; makelock_spec;
@@ -147,6 +99,7 @@ Definition Gprog : funspecs :=
     atomic_load_ptr_spec;
     atomic_store_ptr_spec;
     atomic_CAS_ptr_spec;
+    make_atomic_ptr_spec;
     (* treebox_new_spec; *)
     insert_spec;
     lookup_spec;
